Make progress showing known's approximations OK
Need to strengthen lemma to also include claim that g map approximates
contents of state's globals (assuming that input g0 is related to input
state in same way).

compiler/backend/proofs/clos_knownProofScript.sml
@@ -1,9 +1,18 @@
 open HolKernel Parse boolLib bossLib;
 
 open preamble
-open clos_knownTheory
+open closPropsTheory clos_knownTheory
 
 val _ = new_theory "clos_knownProof";
+
+val bool_case_eq = Q.prove(
+  `COND b t f = v ⇔ b /\ v = t ∨ ¬b ∧ v = f`,
+  srw_tac[][] >> metis_tac[]);
+
+val pair_case_eq = Q.prove (
+`pair_CASE x f = v ⇔ ?x1 x2. x = (x1,x2) ∧ f x1 x2 = v`,
+ Cases_on `x` >>
+ srw_tac[][]);
 
 val known_LENGTH = Q.store_thm(
   "known_LENGTH",
@@ -18,5 +27,197 @@ val known_sing = Q.store_thm(
   qcase_tac `known [e] vs g = (res,g')` >>
   qspecl_then [`[e]`, `vs`, `g`] mp_tac known_LENGTH >> simp[] >>
   Cases_on `res` >> simp[LENGTH_NIL] >> metis_tac[pair_CASES])
+
+val _ = export_rewrites ["closLang.exp_size_def"]
+
+val merge_Impossible = Q.store_thm(
+  "merge_Impossible[simp]",
+  `merge a Impossible = a`,
+  Cases_on `a` >> simp[]);
+
+(* merge defines a meet-semilattice *)
+val merge_comm = Q.store_thm(
+  "merge_comm",
+  `∀a1 a2. merge a1 a2 = merge a2 a1`,
+  ho_match_mp_tac merge_ind >> rpt strip_tac >> simp_tac(srw_ss()) [] >>
+  COND_CASES_TAC >> simp[] >>
+  simp[MAP2_MAP, MAP_EQ_EVERY2, LIST_REL_EL_EQN, EL_ZIP] >>
+  metis_tac[MEM_EL]);
+
+val merge_assoc = Q.store_thm(
+  "merge_assoc",
+  `∀a1 a2 a3. merge a1 (merge a2 a3) = merge (merge a1 a2) a3`,
+  ho_match_mp_tac merge_ind >> rpt strip_tac >> Cases_on `a3` >>
+  simp[] >> rw[LENGTH_MAP2]
+  >- (simp[MAP2_MAP, MAP_EQ_EVERY2, LIST_REL_EL_EQN, EL_ZIP, EL_MAP] >>
+      metis_tac[MEM_EL]) >>
+  rw[])
+
+val merge_idem = Q.store_thm(
+  "merge_idem[simp]",
+  `merge a a = a`,
+  completeInduct_on `val_approx_size a` >> Cases_on `a` >>
+  simp[val_approx_size_def] >> strip_tac >> fs[PULL_FORALL] >>
+  simp[MAP2_MAP, MAP_EQ_ID] >> rpt strip_tac >> first_x_assum match_mp_tac >>
+  rw[] >> Induct_on `l` >> dsimp[val_approx_size_def] >> rpt strip_tac >>
+  res_tac >> simp[]);
+
+val better_defined_approx_def = Define`
+  better_defined_approx a1 a2 ⇔ merge a1 a2 = a1
+`;
+
+val better_defined_approx_refl = Q.store_thm(
+  "better_defined_approx_refl[simp]",
+  `better_defined_approx a a`,
+  simp[better_defined_approx_def]);
+
+val better_definedg_def = Define`
+  better_definedg g1 g2 ⇔
+    ∀k. k ∈ domain g1 ⇒
+        k ∈ domain g2 ∧
+        better_defined_approx (THE (lookup k g1)) (THE (lookup k g2))
+`;
+
+val better_definedg_refl = Q.store_thm(
+  "better_definedg_refl[simp]",
+  `better_definedg g g`,
+  simp[better_definedg_def]);
+
+val va_case_eq =
+    prove_case_eq_thm{case_def = TypeBase.case_def_of ``:val_approx``,
+                      nchotomy = TypeBase.nchotomy_of ``:val_approx``}
+val result_ty = ``:(α,β)semanticPrimitives$result``
+val result_case_eq =
+    prove_case_eq_thm{case_def = TypeBase.case_def_of result_ty,
+                      nchotomy = TypeBase.nchotomy_of result_ty}
+val error_ty = ``:α semanticPrimitives$error_result``
+val error_case_eq =
+    prove_case_eq_thm{case_def = TypeBase.case_def_of error_ty,
+                      nchotomy = TypeBase.nchotomy_of error_ty}
+
+
+val val_approx_val_def = tDefine "val_approx_val" `
+  (val_approx_val (Clos n m) v ⇔ ∃e1 e2 b. v = Closure (SOME n) e1 e2 m b) ∧
+  (val_approx_val (Tuple vas) v ⇔
+    ∃n vs. v = Block n vs ∧ LIST_REL (λv va. val_approx_val v va) vas vs) ∧
+  (val_approx_val Impossible v ⇔ F) ∧
+  (val_approx_val (Int i) v ⇔ v = Number i) ∧
+  (val_approx_val Other v ⇔ T)
+` (WF_REL_TAC `measure (val_approx_size o FST)` >> simp[] >> Induct >>
+   dsimp[val_approx_size_def] >> rpt strip_tac >> res_tac >> simp[])
+
+val val_approx_val_def = save_thm(
+  "val_approx_val_def[simp]",
+  val_approx_val_def |> SIMP_RULE (srw_ss() ++ ETA_ss) []);
+
+val any_el_ALT = Q.store_thm(
+  "any_el_ALT",
+  `∀l n d. any_el n l d = if n < LENGTH l then EL n l else d`,
+  Induct_on `l` >> simp[any_el_def] >> Cases_on `n` >> simp[] >> rw[] >>
+  fs[]);
+
+val merge_Other = Q.store_thm(
+  "merge_Other[simp]",
+  `merge Other a = Other ∧ merge a Other = Other`,
+  Cases_on `a` >> simp[]);
+
+val val_approx_val_merge_I = Q.store_thm(
+  "val_approx_val_merge_I",
+  `∀a1 v a2.
+     val_approx_val a1 v ∨ val_approx_val a2 v ⇒
+     val_approx_val (merge a1 a2) v`,
+  ho_match_mp_tac (theorem "val_approx_val_ind") >>
+  simp[] >> rpt strip_tac >> Cases_on `a2` >> simp[] >> fs[] >> rw[] >>
+  fs[LIST_REL_EL_EQN, LENGTH_MAP2, MAP2_MAP, EL_MAP, EL_ZIP] >>
+  metis_tac[MEM_EL])
+
+val evaluate_list_members_individually = Q.store_thm(
+  "evaluate_list_members_individually",
+  `∀es env (s0:'a closSem$state) vs s.
+     closSem$evaluate (es, env, s0) = (Rval vs, s) ⇒
+     ∀n. n < LENGTH es ⇒
+         ∃(s0':'a closSem$state) s'.
+           evaluate([EL n es], env, s0') = (Rval [EL n vs], s')`,
+  Induct >> simp[] >> Cases_on `es` >> fs[]
+  >- (rpt strip_tac >> qcase_tac `evaluate ([exp], env, _)` >>
+      `∃v. vs = [v]` by metis_tac[evaluate_SING] >> rw[] >> metis_tac[]) >>
+  dsimp[closSemTheory.evaluate_def, pair_case_eq, result_case_eq] >>
+  rpt strip_tac >> reverse (Cases_on `n` >> fs[]) >- metis_tac[] >>
+  imp_res_tac evaluate_SING >> rw[] >> metis_tac[]);
+
+val known_correct_approx = Q.store_thm(
+  "known_correct_approx",
+  `∀es as g0 all g.
+     known es as g0 = (all,g) ⇒
+     ∀e a vs s0 s v.
+        MEM (e,a) all ∧ LIST_REL val_approx_val as vs ∧
+        evaluate([e], vs, s0) = (Rval [v], s) ⇒
+        val_approx_val a v`,
+  ho_match_mp_tac known_ind >> simp[known_def] >> rpt strip_tac
+  >- (qcase_tac `known [exp1] as g0` >>
+      `∃exp1' a1 g1. known [exp1] as g0 = ([(exp1',a1)], g1)`
+         by metis_tac[known_sing] >> fs[] >>
+      qcase_tac `known (exp2::erest) as g1` >>
+      `∃arest g2. known (exp2::erest) as g1 = (arest, g2)`
+         by metis_tac[pair_CASES] >> fs[] >> rw[] >> fs[] >> metis_tac[])
+  >- (fs[any_el_ALT, closSemTheory.evaluate_def, bool_case_eq] >>
+      fs[LIST_REL_EL_EQN])
+  >- (qcase_tac `known [ge] as g0` >>
+      `∃ge' a1 g1. known [ge] as g0 = ([(ge',a1)], g1)`
+         by metis_tac[known_sing] >> fs[] >>
+      qcase_tac `known [tb] as g1` >>
+      `∃tb' a2 g2. known [tb] as g1 = ([(tb',a2)], g2)`
+         by metis_tac[known_sing] >> fs[] >>
+      qcase_tac `known [eb] as g2` >>
+      `∃eb' a3 g3. known [eb] as g2 = ([(eb',a3)], g3)`
+         by metis_tac[known_sing] >> fs[] >> rw[] >> fs[] >> rw[] >>
+      fs[closSemTheory.evaluate_def, pair_case_eq, result_case_eq,
+         bool_case_eq] >> metis_tac[val_approx_val_merge_I])
+  >- ((* let *) qcase_tac `known binds as g0` >>
+      `∃al1 g1. known binds as g0 = (al1,g1)` by metis_tac[pair_CASES] >>
+      fs[] >>
+      qcase_tac `known [bod] (MAP SND al1 ++ as) g1` >>
+      `∃bod' ba g2. known [bod] (MAP SND al1 ++ as) g1 = ([(bod',ba)], g2)`
+        by metis_tac [known_sing] >> fs[] >> rw[] >> fs[] >> rw[] >>
+      fs[closSemTheory.evaluate_def, pair_case_eq, result_case_eq] >> rw[] >>
+      qcase_tac `evaluate (MAP FST al1,vs,s0) = (Rval res1, s1)` >>
+      `LENGTH res1 = LENGTH al1`
+        by (Q.ISPECL_THEN [`MAP FST al1`, `vs`, `s0`] mp_tac
+                          (evaluate_LENGTH |> CONJUNCT1) >> simp[]) >>
+      first_x_assum (qspecl_then [`res1 ++ vs`, `s1`, `s`, `v`] mp_tac) >>
+      impl_tac >> simp[] >> irule EVERY2_APPEND_suff >> simp[] >>
+      simp[LIST_REL_EL_EQN, EL_MAP] >> rpt strip_tac >> first_x_assum irule >>
+      simp[] >>
+      qspecl_then [`MAP FST al1`, `vs`, `s0`, `res1`, `s1`] mp_tac
+        evaluate_list_members_individually >> simp[] >>
+      disch_then (qspec_then `n` mp_tac) >> simp[EL_MAP] >>
+      metis_tac[PAIR, MEM_EL])
+  >- ((* raise *) qcase_tac `known [exp1] as g0` >>
+      `∃exp' ea g1. known [exp1] as g0 = ([(exp',ea)], g1)`
+        by metis_tac [known_sing] >> fs[] >> rw[] >> fs[] >> rw[] >>
+      fs[closSemTheory.evaluate_def, pair_case_eq, result_case_eq])
+  >- ((* tick *) qcase_tac `known [exp1] as g0` >>
+      `∃exp' ea g1. known [exp1] as g0 = ([(exp',ea)], g1)`
+        by metis_tac [known_sing] >> fs[] >> rw[] >> fs[] >> rw[] >>
+      fs[closSemTheory.evaluate_def, pair_case_eq, result_case_eq,
+         bool_case_eq] >> metis_tac[])
+  >- ((* handle *) qcase_tac `known [exp1] as g0` >>
+      `∃exp1' ea1 g1. known [exp1] as g0 = ([(exp1',ea1)], g1)`
+        by metis_tac [known_sing] >> fs[] >> rw[] >>
+      qcase_tac `known [exp2] (Other::as) g1` >>
+      `∃exp2' ea2 g2. known [exp2] (Other::as) g1 = ([(exp2',ea2)], g2)`
+        by metis_tac [known_sing] >> fs[] >> rw[] >> fs[] >> rw[] >>
+      fs[closSemTheory.evaluate_def, pair_case_eq, result_case_eq,
+         error_case_eq] >> rw[] >- metis_tac[val_approx_val_merge_I] >>
+      irule val_approx_val_merge_I >> disj2_tac >> first_x_assum irule >>
+      dsimp[] >> metis_tac[])
+  >- ((* call *) qcase_tac `known exps as g0` >>
+      `∃al1 g1. known exps as g0 = (al1, g1)` by metis_tac[pair_CASES] >>
+      fs[] >> rw[] >> fs[])
+  >> cheat )
+
+
+
+
 
 val _ = export_theory();
